VeriTile/Triton/DSL/Syntax.lean
@@ -144,6 +144,7 @@ syntax:70 tritonExpr:70 " % " tritonExpr:71 : tritonExpr
 syntax ident " := " tritonExpr : tritonStmt
 syntax "tl.store(" tritonExpr ", " tritonExpr ("," tritonMemKwarg)* ")" : tritonStmt
 syntax "tl.atomic_add(" tritonExpr ", " tritonExpr ("," tritonMemKwarg)* ")" : tritonStmt
+syntax "tl.async_copy(" tritonExpr ", " tritonExpr ("," tritonMemKwarg)* ")" : tritonStmt
 syntax "tl.for " ident " in " "$(" term ")" " { " tritonStmt* " }" : tritonStmt
 syntax "tl.for " ident " in " num " { " tritonStmt* " }" : tritonStmt
 syntax "tl.static_range " ident " in " "$(" term ")" " { " tritonStmt* " }" : tritonStmt
